feat(Refinements) add full example using all tools currently available

HOL_To_IMP_Minus/Refinements/HOL_To_IMP_Minus_Datatypes.thy
@@ -1,8 +1,7 @@
 \<^marker>\<open>creator "Kevin Kappelmann"\<close>
 theory HOL_To_IMP_Minus_Datatypes
   imports
-    HOL_To_HOL_Nat.HOL_To_HOL_Nat_Basics
-    HOL_To_IMP_Minus_Primitives
+    HOL_To_IMP_Minus_Arithmetics
 begin
 
 locale HOL_To_HOL_Nat =
@@ -10,55 +9,111 @@ locale HOL_To_HOL_Nat =
   and transport_eq_restrict_id.partial_equivalence_rel_equivalence[per_intro del]
 begin
 
-case_of_simps append_eq_case : append.simps
-function_compile_nat append_eq_case
+fun rev_tail_aux :: "'a list \<Rightarrow> 'a list \<Rightarrow> 'a list" where
+"rev_tail_aux [] acc = acc" |
+"rev_tail_aux (x # xs) acc = rev_tail_aux xs (x # acc)"
 
-case_of_simps rev_eq_case : rev.simps
-function_compile_nat rev_eq_case
+lemma rev_tail_aux_eq_rev_append [simp]: "rev_tail_aux xs acc = rev xs @ acc"
+  by (induction xs arbitrary: acc) auto
+
+case_of_simps rev_tail_aux_eq_case : rev_tail_aux.simps
+function_compile_nat rev_tail_aux_eq_case
+print_theorems
+definition "rev_tail xs \<equiv> rev_tail_aux xs []"
+
+lemma rev_tail_eq_rev [simp]: "rev_tail xs = rev xs"
+  unfolding rev_tail_def by simp
 
 end
+
 context HOL_To_IMP_Minus
 begin
 
-(*dummy stubs; need to compile fst_nat, snd_nat, pair_nat*)
-(*then we could compile constructors and automatically generated functions:*)
-thm Cons_nat_def
+compile_nat Nil_nat_def
+HOL_To_IMP_Minus_correct Nil_nat by cook
+compile_nat Cons_nat_def
+HOL_To_IMP_Minus_correct Cons_nat by cook
 
-declare_compiled_const fst_nat
-  return_register "fst.ret"
-  argument_registers "fst.args.x"
-  compiled suc_IMP
-
-declare_compiled_const snd_nat
-  return_register "fst.ret"
-  argument_registers "fst.args.x"
-  compiled suc_IMP
-
-declare_compiled_const Cons_nat
-  return_register "fst.ret"
-  argument_registers "fst.args.x" "fst.args.y"
-  compiled suc_IMP
-
-declare_compiled_const Pure.type
-  return_register "fst.ret"
-  argument_registers
-  compiled suc_IMP
-
+(*problem: only got a conditional equation. We have to specify an unconditional one and prove it to
+be related to the original HOL function*)
 context
-  fixes xs' ys' :: "('a :: compile_nat) list"
-  assumes rels: "Rel_nat xs xs'" "Rel_nat xs ys'"
+  fixes xs ys and xs' ys' :: "('a :: compile_nat) list"
+  assumes rels: "Rel_nat xs xs'" "Rel_nat ys ys'"
 begin
-
-lemmas test = HOL_To_HOL_Nat.append_nat_eq_unfolded[OF rels, unfolded case_list_nat_def]
-definition "blub x y \<equiv> HOL_To_HOL_Nat.append_nat TYPE('a) x y"
-
-lemma blub_rec: "blub x y =
-  (if fst_nat x = 0 then y else Cons_nat (fst_nat (snd_nat x)) (blub (snd_nat (snd_nat x)) y))"
-  unfolding blub_def by (subst test) (rule refl)
-
-compile_nat blub_rec
-
+term HOL_To_HOL_Nat.rev_tail_aux_nat
+print_statement HOL_To_HOL_Nat.rev_tail_aux_nat_eq_unfolded
+print_statement HOL_To_HOL_Nat.rev_tail_aux_nat_eq_unfolded[OF rels, unfolded case_list_nat_def]
 end
+
+(*FIXME: we could use the equation without unfolding case_list_nat_def if we prove congruence lemmas
+for case_list_nat (otherwise the function package cannot prove termination)*)
+fun rev_tail_aux_nat' :: "nat \<Rightarrow> nat \<Rightarrow> nat" where
+  "rev_tail_aux_nat' xs acc = (if fst_nat xs = 0 then acc else
+    rev_tail_aux_nat' (snd_nat (snd_nat xs)) (Cons_nat (fst_nat (snd_nat xs)) acc))"
+declare rev_tail_aux_nat'.simps[simp del]
+
+compile_nat rev_tail_aux_nat'.simps
+HOL_To_IMP_Minus_correct rev_tail_aux_nat' by (cook mode = tailcall)
+
+(*TODO: how to prove the two functions to be related? Currently, we are missing the right lemmas to
+make it automatic*)
+lemma Rel_nat_NilE:
+  assumes "Rel_nat xs []"
+  obtains "xs = Nil_nat"
+  using assms
+  apply (subst (asm) Rel_nat_iff_eq_natify)
+  apply (subst (asm) natify_list.simps)
+  apply (simp (no_asm_use))
+  by assumption
+
+lemma Rel_nat_ConsE:
+  assumes "Rel_nat xs (y # ys)"
+  obtains z zs where "xs = Cons_nat z zs" "Rel_nat z y" "Rel_nat zs ys"
+  using assms
+  (* apply (subst (asm) (3) Rel_nat_iff_eq_natify)
+  apply (subst (asm) natify_list.simps)
+  apply (simp (no_asm_use))
+  by assumption *)
+  sorry
+
+lemma Rel_nat_NilD:
+  assumes "Rel_nat xs []"
+  shows "xs = Nil_nat"
+  using assms Rel_nat_NilE by blast
+
+lemma Rel_nat_ConsD:
+  assumes "Rel_nat xs (y # ys)"
+  shows "\<exists>z zs. xs = Cons_nat z zs \<and> Rel_nat z y \<and> Rel_nat zs ys"
+  using assms Rel_nat_ConsE by blast
+
+(*probably best approach: use induction on the original function's definition*)
+lemma
+  fixes xs acc and xs' acc' :: "('a :: compile_nat) list"
+  assumes rels: "Rel_nat xs xs'" "Rel_nat acc acc'"
+  shows "Rel_nat (rev_tail_aux_nat' xs acc) (HOL_To_HOL_Nat.rev_tail_aux xs' acc')"
+  using assms
+  apply (induction xs' acc' arbitrary: xs acc rule: HOL_To_HOL_Nat.rev_tail_aux.induct)
+
+  apply (subst HOL_To_HOL_Nat.rev_tail_aux.simps)
+  apply (frule Rel_nat_NilD Rel_nat_ConsD; (elim exE)?)
+  apply hypsubst
+  apply (subst rev_tail_aux_nat'.simps)
+  apply (simp (no_asm) add: Nil_nat_def Cons_nat_def,
+   (simp (no_asm) only: flip: Nil_nat_def Cons_nat_def)?)
+
+  apply (subst HOL_To_HOL_Nat.rev_tail_aux.simps)
+  apply (frule Rel_nat_NilD Rel_nat_ConsD; (elim conjE exE)?)
+  apply hypsubst
+  apply (subst rev_tail_aux_nat'.simps)
+  apply (simp (no_asm) add: Nil_nat_def Cons_nat_def,
+   (simp (no_asm) only: flip: Nil_nat_def Cons_nat_def)?)
+  subgoal premises p
+    apply (rule p(1))
+    apply (insert p(2-))
+    apply (metis Rel_nat_Cons_nat rel_funD)
+    apply (metis Rel_nat_Cons_nat rel_funD)
+    done
+  done
 
 end
 
