HOL_To_IMP_Minus/Refinements/HOL_To_IMP_Minus_Fun_Pattern_Setup.thy
@@ -13,7 +13,7 @@ lemma case_nat_eq_if: "(case n of 0 \<Rightarrow> x | Suc x \<Rightarrow> f x) =
 
 end
 
-paragraph \<open>Example application:\<close>
+paragraph \<open>Example Application\<close>
 
 experiment
 begin
